% !TEX program = xelatex
\documentclass[UTF8]{ctexart}
\usepackage{amsmath}
\usepackage{amssymb}
\usepackage{bm}
\usepackage{geometry}
\usepackage{commath}
\geometry{top = 3cm, bottom = 3cm}
\pagestyle{empty}

\begin{document}
\subsection*{1}
\subsubsection*{(i)}
\begin{align*}
    D &= \left|
    \begin{array}{ccc}
        1 & 0.5 & 0 \\
        -0.5 & 1 & 1.5 \\
        0 & 0 & 1
    \end{array} \right|
    = 1.25 , \\
    D_1& = \left|
    \begin{array}{ccc}
        b_1 & 0.5 & 0 \\
        b_2 & 1 & 1.5 \\
        b_3 & 0 & 1
    \end{array} \right|
    = b_1 - 0.5 b_2 + 0.75 b_3 , \\
    D_2 &= \left|
    \begin{array}{ccc}
        1 & b_1 & 0 \\
        -0.5 & b_2 & 1.5 \\
        0 & b_3 & 1
    \end{array} \right|
    =0.5 b_1 + b_2 - 1.5 b_3 , \\
    D_3 &= \left|
    \begin{array}{ccc}
        1 & 0.5 & b_1 \\
        -0.5 & 1 & b_2 \\
        0 & 0 & b_3
    \end{array} \right|
    = 1.25 b_3.
\end{align*}
Therefore, the solution is
\begin{align*}
    x_1 &= \frac{D_1}{D} = 0.8 b_1 - 0.4 b_2 + 0.6 b_3 , \\
    x_2 &= \frac{D_2}{D} = 0.4 b_1 + 0.8 b_2 - 1.2 b_3 , \\
    x_3 &= \frac{D_3}{D} = b_3 .
\end{align*}

\subsubsection*{(ii)}
\[
    \left( \begin{array}{ccc}
        1 & 0.5 & 0 \\
        -0.5 & 1 & 1.5 \\
        0 & 0 & 1
    \end{array} \right)
    \left( \begin{array}{c}
        x_1 \\ x_2 \\ x_3
    \end{array} \right)
    =
    \left( \begin{array}{c}
        b_1 \\ b_2 \\ b_3
    \end{array} \right)
\]

\subsubsection*{(iii)}
\[
    A^{-1} = \frac{1}{5} \left(
    \begin{array}{ccc}
        4 & -2 & 3 \\
        2 & 4 & -6 \\
        0 & 0 & 5
    \end{array}
    \right)
\]
It is easy to get $A^{-1} \bm{b} = \bm{x}$.

\subsection*{2}
\[
    f_x(x, y) = 4 x^{-\frac{1}{3}} y^{\frac{1}{2}}
    \qquad\qquad\qquad
    f_y(x, y) = 3 x^{\frac{2}{3}} y^{-\frac{1}{2}}
\]
Let $x_0 = 1000, y_0 = 100$ , we can estimate the function value
\begin{align*}
    f(998, 101.5)
    &= f(x_0, y_0) + f_x(x_0, y_0) (998 - x_0) + f_y(x_0, y_0) (101.5 - y_0) \\
    &= 6000 - 4 \times 2 + 30 \times 1.5
    = 6037
\end{align*}

\subsection*{3}
Let $f(x, y) = x^2 - 3xy + y^3 - 7$ .
\subsubsection*{(i)}
$f(4, 3) = 0$ , so the point $(4,3)$ is on the curve defined by the equation.
\subsubsection*{(ii)}
\begin{gather*}
    \frac{\dif y}{\dif x} =
    - \frac{f_x}{f_y} =
    \frac{2x - 3y}{3x - 3y^2} \ ,\; 
    \frac{\dif y}{\dif x} \bigg|_{(4, 3)} = \frac{1}{15}
\end{gather*}
\subsubsection*{(iii)}
Suppose the implicit function decided by the equation is $y = g(x)$ , and $g(4) = 3$ . Therefore, we have
\[
    \Delta g_1 = g(4.1) - g(4)
    \approx g(4) + \frac{\dif y}{\dif x} \bigg|_{x = 4} (4.1 - 4) - g(4) = \frac{1}{150}
\]
Using the computer, I get that $\Delta y_2 = 0.0061 > \Delta y_1$ .

\subsection*{4}
Let $F(x, y) = f(x, y) + g(y) - y + z$ .
\subsubsection*{(i)}
\begin{align*}
    \frac{\dif y}{\dif x} = -\frac{F_x}{F_y}
    = - \frac{f_x}{f_y + g' - 1}
\end{align*}
\[
    \begin{cases}
        \Delta y = \dfrac{\dif y}{\dif x} \Delta x \\
        \Delta m = m_x \Delta x + m_y \Delta y
    \end{cases}
    \Longrightarrow\;
    \Delta x = \frac{f_y + g' - 1}{m_x (f_y + g' - 1) - m_y f_x} \Delta m
\]
\subsubsection*{(ii)}
Consider $Z(x, y) = y - f(x, y) - g(y)$ , then
\[
    \begin{cases}
        \Delta z = - f_x \Delta x + (1 - f_y - g')\Delta y \\
        0 = \Delta m = m_x \Delta x + m_y \Delta y
    \end{cases}
    \Longrightarrow\;
    \Delta y = \frac{m_x}{m_x (1 - f_y - g') + m_y f_x} \Delta z
\]
\end{document}