\documentclass{article}
\usepackage{amsmath}
\usepackage{geometry}
\usepackage{commath}

\pagestyle{empty}

\renewcommand{\thesection}{\arabic{section}.}
\renewcommand{\thesubsection}{(\alph{subsection})}
\newcommand{\kast}{k^\ast}

\begin{document}
\section{}
\subsection{}
As the Solow Model without technological progrss, in which
\[
    \dot{L_t} = n L_t \qquad\qquad
    \dot{K_t} = sY - \delta K_t,
\]
in the model with technological progrss, we also have
\[
    \dot{E_t} = g E_t
\]
and define
\[
    f(k_t) \equiv y_t = \frac{Y_t}{E_t L_t}
    = K_t^\alpha (E_t L_t)^{-\alpha} = k_t^\alpha.
\]
Therefore, 
\[
    \dot{k_t} = \frac{\dif}{\dif t} \left( \frac{K_t}{E_t L_t} \right)
    %= \frac{\dot{K_t} E_t L_t - K_t (\dot{E_t} L_t + E_t \dot{L_t})}{(E_t L_t)^2}
    = s f(k_t) - (\delta + g + n) k_t
    = s k_t^\alpha - (\delta + g + n) k_t.
\]
When the steady state is reached,
\[
    \dot{k_t}|_{k_t = \kast} = 0 \,\Longrightarrow\,
    \kast = \left( \frac{\delta + g + n}{s} \right)^{\frac{1}{\alpha - 1}}.
\]
Plug the $\kast$ into the expressions, we have
\begin{align*}
    y^\ast &= f(\kast) = \left( \frac{\delta + g + n}{s} \right)^{\frac{\alpha}{\alpha - 1}}, \\
    c^\ast &= (1-s) y^\ast = (1-s) \left( \frac{\delta + g + n}{s} \right)^{\frac{\alpha}{\alpha - 1}}.
\end{align*}

\subsection{}
To maximize the $c^\ast = y^\ast - s y^\ast 
= (\kast)^\alpha - (\delta + g + n) \kast$, employ the FOC and get
\[
    \frac{\partial c^\ast}{\partial \kast} \bigg|_{\kast = \kast_g} = 0
    \,\Longrightarrow\,
    \kast_g = \left( \frac{\delta + g + n}{\alpha} \right)^{\frac{1}{\alpha - 1}}.
\]    

\subsection{}
To find the the golden-rule saving rate, just let $\kast = \kast_g$ and solve it. Since $\partial \kast / \partial s > 0$,
\[
    s_g = \alpha.
\]

\section{}
\subsection{}
\begin{align*}
    MPK &= \frac{\partial Y_t}{\partial K_t}
    = \frac{\partial}{\partial K_t} \left(E_t L_t \cdot f\Big( \frac{K_t}{E_t L_t} \Big)\right) \\
    &= \frac{\partial }{\partial (K_t / (E_t L_t))} f\Big( \frac{K_t}{E_t L_t} \Big) \\
    &= f' \left( \frac{K_t}{E_t L_t} \right)
    = f'(k)
\end{align*}
When at the steady state, $k = \kast$. That is, $MPK \big|_{k = \kast} = f'(\kast)$.

\subsection{}
Despite the change of distribution, the equation of the dynamics of p.e.w. capital accumulation still works,
\[
    \dot{k_t} = \frac{\dif}{\dif t} \left( \frac{K_t}{E_t L_t} \right)
    = \frac{\dot{K_t} E_t L_t - K_t (\dot{E_t} L_t + E_t \dot{L_t})}{(E_t L_t)^2}.
\]
Plugging the new expression of $\dot{K_t}$ into the equation, we have
\begin{align}
    \dot{k_t} &= (MPK - \delta) k_t - (g + n) k_t
    = k_t \cdot f'(k_t) - (\delta + g + n) k_t. \label{d}
\end{align}

\subsection{}
According to \eqref{d}, at he steady state,
\[
    \dot{k_t} = 0 \,\Longrightarrow\,
    f'(k_t) = \delta + g + n.
\]
Meanwhile, $c^\ast = y^\ast - s y^\ast = f(\kast) - (\delta + g + n) \kast$. Employ the FOC and we can compute that the golden-rule level of capital per capita satisfies
\[
    f'(\kast_g) = \delta + g + n.
\]
In the model assumption, $f''(k) < 0$. Therefore, $\kast = \kast_g$.

\end{document}